Temporal_Planning_Base/Temporal_Plans.thy
@@ -1,5 +1,5 @@
 theory Temporal_Plans
-  imports Base
+  imports Base "Difference_Bound_Matrices.DBM"
 begin
 
 datatype ('t) lower_bound =
